iris/SpecKexecB3.v
@@ -139,7 +139,7 @@ Definition kxc_b2_body
                  (m !!! Regidx Rs3) (m !!! Regidx Rs4) (m !!! Regidx Rs5)
                  (m !!! Regidx Rs6) (m !!! Regidx Rs7) (m !!! Regidx Rs8)
                  (m !!! Regidx Rs9) (m !!! Regidx Rs10) (m !!! Regidx Rs11)
-                 w67 ef P' Mo szv' (m !!! Regidx Rs11) -∗
+                 w67 (kxc_fb datl dnf) ef P' Mo szv' (m !!! Regidx Rs11) -∗
       wp_next (CID0 := CID) true (proc_addr jp) (fun (CIDy : CpuId) =>
         KexecOkQ.kexec_closer Q gf fsc_kalloc (proc_addr jp) pidv U m (ret_pc ra0) K
              eb eb ∅ dqb dqs fsc_bmapstart na alen plen pv dqpv
@@ -196,7 +196,8 @@ Definition kxc_b2z_body
                  (m !!! Regidx Rs3) (m !!! Regidx Rs4) (m !!! Regidx Rs5)
                  (m !!! Regidx Rs6) (m !!! Regidx Rs7) (m !!! Regidx Rs8)
                  (m !!! Regidx Rs9) (m !!! Regidx Rs10) w13
-                 w67 ef P Mi (mword_of_int 0 : mword 64) (m !!! Regidx Rs11) -∗
+                 w67 (kxc_fb datl dnf) ef P Mi
+                 (mword_of_int 0 : mword 64) (m !!! Regidx Rs11) -∗
       WP (Loop : expr riscv_lang)) -∗
   WP (Loop : expr riscv_lang).
 
